examples/cannon/CannonMainIAproof.v
@@ -14,11 +14,10 @@ Module CannonMainIA. Section CannonMainIA.
   Definition Ist : nat → alist key Any.t → alist key Any.t → iProp Σ :=
     λ _ _ _, (True)%I.
 
-  Variable ginv : invspec.
   Variable SpcMain : string → option fspec.
   Hypothesis CannonInSpcMain : spc_incl CannonAS.Spc SpcMain.
   
-  Local Notation MainAMod := (MainA.t 1 ginv SpcMain).
+  Local Notation MainAMod := (MainA.t 1 SpcMain).
   Local Notation MainIMod := (MainI.t 1).
   
   Lemma simF_main : HSim.sim_fun open MainAMod MainIMod Ist MainName.main.
