examples/mutsum/MutFA.v
@@ -35,5 +35,5 @@ Module MutFA. Section MutFA.
 
   Definition InitCond : iProp := emp%I.
 
-  Definition t ginv Spc := Seal.sealing CRIS (SMod.to_hmod ginv Spc Mod).
+  Definition t Spc := Seal.sealing CRIS (SMod.to_hmod ginv_emp Spc Mod).
 End MutFA. End MutFA.
