examples/repeat/AddA.v
@@ -63,5 +63,5 @@ Module AddA. Section AddA.
 
   Definition InitCond : iProp Σ := emp%I.
 
-  Definition t ginv Spc := Seal.sealing CRIS (SMod.to_hmod ginv Spc Mod).
+  Definition t Spc := Seal.sealing CRIS (SMod.to_hmod ginv_emp Spc Mod).
 End AddA. End AddA.
